Examples/dlist.v
@@ -2,7 +2,7 @@
 From Coq Require Import ssreflect ssrbool ssrfun.
 From mathcomp Require Import ssrnat eqtype seq.
 From fcsl Require Import axioms pred.
-From fcsl Require Import pcm unionmap heap automap.
+From fcsl Require Import pcm unionmap heap auto autopcm.
 From HTT Require Import model heapauto.
 Set Implicit Arguments.
 Unset Strict Implicit.
@@ -235,7 +235,7 @@ move=>p _ go [r acc] _ _ [->->][l][nx][] i /= H; case: ifP H=>[/eqP->|/negbT].
 (* deconstruct non-empty remainder *)
 rewrite eq_sym=>Hr /(dseg_neqR Hr) [xs][x][z][h'][{l}-> {i}-> H'].
 (* run the rest, feed remainder, acc pointer and subheap to recursive call *)
-do 2!step; apply: [gR xs, r]@h'=>//= _ m [Hm ->] _ /=.
+do 2!step; apply: [gX xs, r]@h'=>//= _ m [Hm ->] _ /=.
 (* simplify and restructure the goal *)
 split; last by rewrite -cats1 -catA.
 by apply/dseg_rcons; vauto.
